Generate vale stub for stack args

src/arch/x64/Interop.fst
@@ -10,6 +10,7 @@ module List = FStar.List.Tot.Base
 module HS = FStar.Monotonic.HyperStack
 module HH = FStar.Monotonic.HyperHeap
 module B = LowStar.Buffer
+module M = LowStar.Modifies
 
 open Opaque_s
 open X64.Machine_s
@@ -23,6 +24,8 @@ let op_String_Assignment = Map.upd
 
 let sub l i = l - i
 
+let b8 = B.buffer UInt8.t
+
 unfold
 let disjoint_or_eq ptr1 ptr2 = B.disjoint ptr1 ptr2 \/ ptr1 == ptr2
 
@@ -33,15 +36,21 @@ let disjoint_addr addr1 length1 addr2 length2 =
   (* The first buffer is completely before the second, or the opposite *)
   addr1 + length1 < addr2 || addr2 + length2 < addr1
 
-type addr_map = (m:((B.buffer UInt8.t) -> nat64){
-  (forall (buf1 buf2:B.buffer UInt8.t). B.disjoint buf1 buf2 ==> 
+type addr_map = (m:(b8 -> nat64){
+  (forall (buf1 buf2:b8). B.disjoint buf1 buf2 ==> 
     disjoint_addr (m buf1) (B.length buf1) (m buf2) (B.length buf2)) /\
-  (forall (b:B.buffer UInt8.t). m b + B.length b < pow2_64)})
+  (forall (b:b8). m b + B.length b < pow2_64)})
 
 unfold
 let list_live mem ptrs = forall p . List.memP p ptrs ==> B.live mem p
 
 (* Additional hypotheses, which should be added to the corresponding libraries at some point *)
+
+//This lemma will be available in the next version of Low*
+assume val buffers_disjoint (b1 b2:b8) : Lemma
+  (requires M.loc_disjoint (M.loc_buffer b1) (M.loc_buffer b2))
+  (ensures B.disjoint b1 b2)
+  [SMTPat (B.disjoint b1 b2)]
 
 (* If two refs have the same address, and are in the heap, they are equal *)
 assume val ref_extensionality (#a:Type0) (#rel:Preorder.preorder a) (h:Heap.heap) (r1 r2:Heap.mref a rel) : Lemma 
@@ -90,7 +99,7 @@ let rec load_store_write_vale_mem
 	load_store_write_vale_mem contents length addr (i+1) heap
       end
 
-let correct_down_p (mem:HS.mem) (addrs:addr_map) (heap:heap) (p:B.buffer UInt8.t) =
+let correct_down_p (mem:HS.mem) (addrs:addr_map) (heap:heap) (p:b8) =
   let length = B.length p in
   let contents = B.as_seq mem p in
   let addr = addrs p in
@@ -98,14 +107,14 @@ let correct_down_p (mem:HS.mem) (addrs:addr_map) (heap:heap) (p:B.buffer UInt8.t
 
 #set-options "--z3rlimit 40"
 
-let correct_down_p_cancel mem (addrs:addr_map) heap (p:B.buffer UInt8.t) : Lemma
+let correct_down_p_cancel mem (addrs:addr_map) heap (p:b8) : Lemma
   (forall p'. p == p' ==>       
       (let length = B.length p in
       let contents = B.as_seq mem p in
       let addr = addrs p in
       let new_heap = write_vale_mem contents length addr 0 heap in
       correct_down_p mem addrs new_heap p')) = 
-  let rec aux (p':B.buffer UInt8.t) : Lemma 
+  let rec aux (p':b8) : Lemma 
     (p == p'  ==> (let length = B.length p in
       let contents = B.as_seq mem p in
       let addr = addrs p in
@@ -119,14 +128,14 @@ let correct_down_p_cancel mem (addrs:addr_map) heap (p:B.buffer UInt8.t) : Lemma
   in
   Classical.forall_intro aux
       
-let correct_down_p_frame mem (addrs:addr_map) (heap:heap) (p:B.buffer UInt8.t) : Lemma
+let correct_down_p_frame mem (addrs:addr_map) (heap:heap) (p:b8) : Lemma
   (forall p'. B.disjoint p p' /\ correct_down_p mem addrs heap p' ==>       
       (let length = B.length p in
       let contents = B.as_seq mem p in
       let addr = addrs p in
       let new_heap = write_vale_mem contents length addr 0 heap in
       correct_down_p mem addrs new_heap p')) = 
-  let rec aux (p':B.buffer UInt8.t) : Lemma 
+  let rec aux (p':b8) : Lemma 
     (B.disjoint p p' /\ correct_down_p mem addrs heap p' ==> (let length = B.length p in
       let contents = B.as_seq mem p in
       let addr = addrs p in
@@ -140,17 +149,17 @@ let correct_down_p_frame mem (addrs:addr_map) (heap:heap) (p:B.buffer UInt8.t) :
   in
   Classical.forall_intro aux
 
-let correct_down mem (addrs:addr_map) (ptrs: list (B.buffer UInt8.t)) heap =
+let correct_down mem (addrs:addr_map) (ptrs: list b8) heap =
   forall p. List.memP p ptrs ==> correct_down_p mem addrs heap p
 
 (* Takes a Low* Hyperstack and two buffers (for the moment) and create a vale memory + keep track of the vale addresses *)
-val down_mem: (mem:HS.mem) -> (addrs: addr_map) -> (ptrs:list (B.buffer UInt8.t){list_disjoint_or_eq ptrs}) -> GTot (heap :heap {correct_down mem addrs ptrs heap})
+val down_mem: (mem:HS.mem) -> (addrs: addr_map) -> (ptrs:list b8{list_disjoint_or_eq ptrs}) -> GTot (heap :heap {correct_down mem addrs ptrs heap})
 
-let rec down_mem_aux (ptrs:list (B.buffer UInt8.t){list_disjoint_or_eq ptrs})
+let rec down_mem_aux (ptrs:list b8{list_disjoint_or_eq ptrs})
   (addrs:addr_map)
   (mem:HS.mem)
-  (ps:list (B.buffer UInt8.t))
-  (accu:list (B.buffer UInt8.t){forall p. List.memP p ptrs <==> List.memP p ps \/ List.memP p accu})
+  (ps:list b8)
+  (accu:list b8{forall p. List.memP p ptrs <==> List.memP p ps \/ List.memP p accu})
   (h:heap{correct_down mem addrs accu h}) : 
   GTot (heap:heap{correct_down mem addrs ptrs heap}) =
   match ps with
@@ -176,26 +185,26 @@ let down_mem mem addrs ptrs =
 val unspecified_down:
   (mem:HS.mem) ->
   (addrs:addr_map) ->
-  (ptrs: list (B.buffer UInt8.t){list_disjoint_or_eq ptrs}) ->
+  (ptrs: list b8{list_disjoint_or_eq ptrs}) ->
   Lemma (
     let heap = down_mem mem addrs ptrs in
     forall i. (
-      forall (b:B.buffer UInt8.t{List.memP b ptrs}).
+      forall (b:b8{List.memP b ptrs}).
         let base = addrs b in
 	i < base \/ i >= base + B.length b) ==>
       heap.[i] == 0)
 
 private
 let rec frame_down_mem_aux
-  (ptrs:list (B.buffer UInt8.t){list_disjoint_or_eq ptrs})
+  (ptrs:list b8{list_disjoint_or_eq ptrs})
   (addrs:addr_map)
   (mem:HS.mem)
-  (ps:list (B.buffer UInt8.t))
-  (accu: list (B.buffer UInt8.t){forall p. List.memP p ptrs <==> List.memP p ps \/ List.memP p accu})
+  (ps:list b8)
+  (accu: list b8{forall p. List.memP p ptrs <==> List.memP p ps \/ List.memP p accu})
   (h:heap{correct_down mem addrs accu h}) :
   Lemma (
     let heap = down_mem_aux ptrs addrs mem ps accu h in
-    forall i. (forall (b:B.buffer UInt8.t{List.memP b ps}).
+    forall i. (forall (b:b8{List.memP b ps}).
       let base = addrs b in
       i < base \/ i >= base + B.length b) ==>
     heap.[i] == h.[i]) =
@@ -223,11 +232,11 @@ val same_unspecified_down:
   (mem1: HS.mem) -> 
   (mem2: HS.mem) -> 
   (addrs:addr_map) ->
-  (ptrs:list (B.buffer UInt8.t){list_disjoint_or_eq ptrs}) ->
+  (ptrs:list b8{list_disjoint_or_eq ptrs}) ->
   Lemma (
     let heap1 = down_mem mem1 addrs ptrs in
     let heap2 = down_mem mem2 addrs ptrs in
-    forall i. (forall (b:B.buffer UInt8.t{List.memP b ptrs}). 
+    forall i. (forall (b:b8{List.memP b ptrs}). 
       let base = addrs b in
       i < base \/ i >= base + B.length b) ==>
       heap1.[i] == heap2.[i])
